SeparationLogic/DeepEmbedded/ParametricSeparationLogic.v
@@ -1,15 +1,15 @@
 Require Import Logic.GeneralLogic.Base.
 Require Import Logic.MinimunLogic.Syntax.
-Require Import Logic.PropositionalLogic.Syntax.
-Require Import Logic.SeparationLogic.Syntax.
-Require Import Logic.MinimunLogic.ProofTheory.Normal.
 Require Import Logic.MinimunLogic.ProofTheory.Minimun.
 Require Import Logic.MinimunLogic.ProofTheory.RewriteClass.
+Require Import Logic.MinimunLogic.Syntax.
+Require Import Logic.MinimunLogic.ProofTheory.Minimun.
+Require Import Logic.PropositionalLogic.Syntax.
 Require Import Logic.PropositionalLogic.ProofTheory.Intuitionistic.
 Require Import Logic.PropositionalLogic.ProofTheory.DeMorgan.
 Require Import Logic.PropositionalLogic.ProofTheory.GodelDummett.
 Require Import Logic.PropositionalLogic.ProofTheory.Classical.
-Require Import Logic.PropositionalLogic.ProofTheory.RewriteClass.
+Require Import Logic.SeparationLogic.Syntax.
 Require Import Logic.SeparationLogic.ProofTheory.SeparationLogic.
 Require Import Logic.SeparationLogic.DeepEmbedded.Parameter.
 Require Logic.SeparationLogic.DeepEmbedded.SeparationEmpLanguage.
@@ -19,24 +19,20 @@ Local Open Scope syntax.
 Import PropositionalLanguageNotation.
 Import SeparationLogicNotation.
 
-Class Parametric_SeparationLogic (PAR: SL_Parameter) (L: Language) {nL: NormalLanguage L} {pL: PropositionalLanguage L} {sL: SeparationLanguage L} {s'L: SeparationEmpLanguage L} (Gamma: ProofTheory L) {nGamma: NormalProofTheory L Gamma} {mpGamma: MinimunPropositionalLogic L Gamma} {ipGamma: IntuitionisticPropositionalLogic L Gamma} {sGamma: SeparationLogic L Gamma} {eGamma: EmpSeparationLogic L Gamma} := {
-  Parametric_DM: WEM PAR = true -> DeMorganPropositionalLogic L Gamma;
-  Parametric_GD: IC PAR = true -> GodelDummettPropositionalLogic L Gamma;
-  Parametric_C: EM PAR = true -> ClassicalPropositionalLogic L Gamma;
-  Parametric_GC: SCE PAR = true -> GarbageCollectSeparationLogic L Gamma;
-  Parametric_NE: ESE PAR = true -> NonsplitEmpSeparationLogic L Gamma;
-  Parametric_ED: ED PAR = true -> DupEmpSeparationLogic L Gamma
+Class Parametric_SeparationLogic (PAR: SL_Parameter) (L: Language) {minL: MinimunLanguage L} {pL: PropositionalLanguage L} {sL: SeparationLanguage L} {s'L: SeparationEmpLanguage L} (Gamma: ProofTheory L) {AX: NormalAxiomatization L Gamma} {minAX: MinimunAxiomatization L Gamma} {ipGamma: IntuitionisticPropositionalLogic L Gamma} {sGamma: SeparationLogic L Gamma} {eGamma: EmpSeparationLogic L Gamma} := {
+  Parametric_DM: WEM = true -> DeMorganPropositionalLogic L Gamma;
+  Parametric_GD: IC = true -> GodelDummettPropositionalLogic L Gamma;
+  Parametric_C: EM = true -> ClassicalPropositionalLogic L Gamma;
+  Parametric_GC: SCE = true -> GarbageCollectSeparationLogic L Gamma;
+  Parametric_NE: ESE = true -> NonsplitEmpSeparationLogic L Gamma;
+  Parametric_ED: ED = true -> DupEmpSeparationLogic L Gamma
 }.
 
 Section SeparationLogic.
 
-Context (Var: Type).
+Context {Sigma: SeparationEmpLanguage.PropositionalVariables}.
 
-Instance L: Language := SeparationEmpLanguage.L Var.
-Instance nL: NormalLanguage L := SeparationEmpLanguage.nL Var.
-Instance pL: PropositionalLanguage L := SeparationEmpLanguage.pL Var.
-Instance sL: SeparationLanguage L := SeparationEmpLanguage.sL Var.
-Instance s'L: SeparationEmpLanguage L := SeparationEmpLanguage.s'L Var.
+Existing Instances SeparationEmpLanguage.L SeparationEmpLanguage.minL SeparationEmpLanguage.pL SeparationEmpLanguage.sL SeparationEmpLanguage.s'L.
 
 Context (PAR: SL_Parameter).
 
@@ -51,23 +47,23 @@ Inductive provable: expr -> Prop :=
 | orp_intros2: forall x y, provable (y --> x || y)
 | orp_elim: forall x y z, provable ((x --> z) --> (y --> z) --> (x || y --> z))
 | falsep_elim: forall x, provable (FF --> x)
-| weak_excluded_middle: WEM PAR = true -> forall x, provable (~~ x || ~~ ~~ x)
-| impp_choice: IC PAR = true -> forall x y, provable ((x --> y) || (y --> x))
-| excluded_middle: EM PAR = true -> forall x, provable (x || ~~ x)
+| weak_excluded_middle: WEM = true -> forall x, provable (~~ x || ~~ ~~ x)
+| impp_choice: IC = true -> forall x y, provable ((x --> y) || (y --> x))
+| excluded_middle: EM = true -> forall x, provable (x || ~~ x)
 | sepcon_comm: forall x y, provable (x * y --> y * x)
 | sepcon_assoc: forall x y z, provable (x * (y * z) <--> (x * y) * z)
 | wand_sepcon_adjoint1: forall x y z, provable (x * y --> z) -> provable (x --> (y -* z))
 | wand_sepcon_adjoint2: forall x y z, provable (x --> (y -* z)) -> provable (x * y --> z)
 | sepcon_emp: forall x, provable (x * emp <--> x)
-| sepcon_elim1: SCE PAR = true -> forall x y, provable (x * y --> x)
-| emp_sepcon_truep_elim: ESE PAR = true -> forall x, provable (x * TT && emp --> x)
-| emp_dup: ED PAR = true -> forall x, provable (x && emp --> x * x).
+| sepcon_elim1: SCE = true -> forall x y, provable (x * y --> x)
+| emp_sepcon_truep_elim: ESE = true -> forall x, provable (x * TT && emp --> x)
+| emp_dup: ED = true -> forall x, provable (x && emp --> x * x).
 
-Instance G: ProofTheory L := Build_AxiomaticProofTheory provable.
+Instance G: ProofTheory SeparationEmpLanguage.L := Build_AxiomaticProofTheory provable.
 
-Instance nG: NormalProofTheory L G := Build_nAxiomaticProofTheory provable.
+Instance AX: NormalAxiomatization SeparationEmpLanguage.L G := Build_AxiomaticProofTheory_AX provable.
 
-Instance mpG: MinimunPropositionalLogic L G.
+Instance minAX: MinimunAxiomatization SeparationEmpLanguage.L G.
 Proof.
   constructor.
   + apply modus_ponens.
@@ -75,7 +71,7 @@ Proof.
   + apply axiom2.
 Qed.
 
-Instance ipG: IntuitionisticPropositionalLogic L G.
+Instance ipG: IntuitionisticPropositionalLogic SeparationEmpLanguage.L G.
 Proof.
   constructor.
   + apply andp_intros.
@@ -87,7 +83,7 @@ Proof.
   + apply falsep_elim.
 Qed.
 
-Instance sG: SeparationLogic L G.
+Instance sG: SeparationLogic SeparationEmpLanguage.L G.
 Proof.
   constructor.
   + apply sepcon_comm.
@@ -97,14 +93,14 @@ Proof.
     - apply wand_sepcon_adjoint2.
 Qed.
 
-Instance eG: EmpSeparationLogic L G.
+Instance eG: EmpSeparationLogic SeparationEmpLanguage.L G.
 Proof.
   constructor.
   intros.
   apply sepcon_emp.
 Qed.
 
-Instance ParG: Parametric_SeparationLogic PAR L G.
+Instance ParG: Parametric_SeparationLogic PAR SeparationEmpLanguage.L G.
 Proof.
   constructor.
   + intros; constructor.
